change NULL to be the NULLptr

smonad/lists.v
@@ -4,15 +4,13 @@ Require Import List.
 Require Import Omega.
 
 Inductive SLL (A:Set) : Set :=
-| NULL : SLL A
 | NODE : A -> Addr -> SLL A.
 Hint Constructors SLL.
 
 Inductive SLL_is_List (A:Set) : (Memory (SLL A)) -> Addr -> (list A) -> Prop :=
 | SiL_nil :
-  forall mem a,
-    mem_map (SLL A) mem a = Some (NULL A) ->
-    SLL_is_List A mem a nil
+  forall mem,
+    SLL_is_List A mem NULLptr nil
 | SiL_cons :
   forall mem a v l' a',
     SLL_is_List A mem a' l' ->
@@ -22,12 +20,13 @@ Hint Constructors SLL_is_List.
 
 Lemma SLL_is_List_fun:
   forall A mem a l1,
+    Memory_Valid (SLL A) mem ->
     SLL_is_List A mem a l1 ->
     forall l2,
       SLL_is_List A mem a l2 ->
       l1 = l2.
 Proof.
-  intros A mem a l1 S1;
+  intros A mem a l1 [EQnp MV] S1;
     induction S1; intros l2 S2;
       inversion S2.
 
@@ -43,20 +42,20 @@ Qed.
 
 Lemma memory_extends_SLL:
   forall A mem a' l,
+    Memory_Valid (SLL A) mem ->
     SLL_is_List A mem a' l ->
     forall a v mem',
       Memory_Extends (SLL A) mem a v mem' ->
       SLL_is_List A mem' a' l.
 Proof.
-  intros A mem a' n SiL.
+  intros A mem a' n MV SiL.
   induction SiL as [mem a' MS|mem a' v' l' a'' SiL MS];
     intros a v mem' ME.
 
-  unfold Memory_Extends in ME.
-  eapply SiL_nil. intuition.
+  eapply SiL_nil. 
 
   eapply (SiL_cons _ _ _ _ _ a'').
-  eapply MS. apply ME.
+  eapply MS. auto. apply ME.
   unfold Memory_Extends in ME.
   intuition.
 Qed.
@@ -81,7 +80,12 @@ Program Fixpoint memory_list_of_len (n:nat) :
   (@inc _ 1 _ _ _
     (match n with
        | O =>
-         (@weaken _ _ _ _ _ _ (@malloc (SLL nat) (NULL nat)) _ _)
+         (@weaken _ _ _ _ _ _
+           (@ret _ _ (fun mem a an mem' =>
+             an = 0 /\
+             mem' = mem /\
+             SLL_is_List _ mem' a (list_of_len n))
+           NULLptr _) _ _)
        | S m =>
          (@weaken _ _ _ _ _ _
            (@bind _ _ _ _
@@ -101,28 +105,25 @@ Program Fixpoint memory_list_of_len (n:nat) :
      end)).
 
 Next Obligation.
-  rename H2 into ME.
-  unfold Memory_Extends in ME.
-  split. auto.
-  split. intuition.
-  eapply SiL_nil.
-  intuition.
+  simpl. auto.
 Defined.
 
 Next Obligation.
-  rename H4 into ME.
+  rename H5 into ME.
   rename H2 into SiLst.
+  rename H1 into MVst.
   split. auto.
   split. unfold Memory_Extends in ME. intuition.
   eapply (SiL_cons _ st' (mem_next (SLL _) st) m _ a');
     try (intuition; fail).
   eapply memory_extends_SLL.
+  apply MVst.
   apply SiLst. apply ME.
   unfold Memory_Extends in ME. intuition.
 Defined.
 
 Next Obligation.
-  rename H1 into EQm.
+  rename H2 into EQm.
   rewrite EQm.
   split. omega.
   auto.
@@ -138,9 +139,7 @@ Proof.
   generalize mem' MLE. clear mem' MLE.
   induction SiL; intros mem' MLE.
 
-  rename H into MS.
-  eapply SiL_nil.
-  apply (Memory_le_Same (SLL A) mem mem' MLE a _ MS).
+  auto.
 
   rename H into MS.
   eapply SiL_cons.
@@ -150,10 +149,9 @@ Qed.
 
 Inductive SLL_lt_core (A:Set) (mem:Memory (SLL A)) : Addr -> Addr -> Prop :=
 | Sltc_NULL :
-  forall to from v,
-    mem_map (SLL A) mem to = Some (NULL A) ->
-    mem_map (SLL A) mem from = Some (NODE A v to) ->
-    SLL_lt_core A mem to from
+  forall from v,
+    mem_map (SLL A) mem from = Some (NODE A v NULLptr) ->
+    SLL_lt_core A mem NULLptr from
 | Sltc_NODE :
   forall to next from v v',
     (* This ensures that there is no cycle, because Coq won't let us
@@ -167,9 +165,10 @@ Hint Constructors SLL_lt_core.
 Definition SLL_lt (A:Set) (mem_to:((Memory (SLL A))*Addr))
   (mem_from:((Memory (SLL A))*Addr)) :=
   let (mem', to) := mem_to in
-  let (mem, from) := mem_from in
-    Memory_le (SLL A) mem mem' /\
-    SLL_lt_core A mem to from.
+    let (mem, from) := mem_from in
+      Memory_Valid (SLL A) mem /\
+      Memory_le (SLL A) mem mem' /\
+      SLL_lt_core A mem to from.
 Hint Unfold SLL_lt.
 
 Theorem SLL_lt_wf:
@@ -182,30 +181,29 @@ Proof.
 
   unfold SLL_lt in *; simpl in *.
 
-  destruct Slt1 as [MLE1 Sltc1].
-  generalize mem' MLE1.
-  clear mem' MLE1.
-  induction Sltc1; intros mem' MLE1.
+  destruct Slt1 as [MV1 [MLE1 Sltc1]].
+  generalize mem' MV1 MLE1.
+  clear mem' MV1 MLE1.
+  induction Sltc1; intros mem' MV1 MLE1.
 
-  rename to into to1.
   rename from into from1.
-  rename H into MS_to1.
-  rename H0 into MS_from1.
+  rename H into MS_from1.
   eapply Acc_intro.
   intros [mem2 to2] Slt2.
-  destruct Slt2 as [MLE2 Sltc2].
+  destruct Slt2 as [MV2 [MLE2 Sltc2]].
   inversion Sltc2; clear Sltc2.
-  subst to from.
-  rename H into MS_to2.
-  rename H0 into MS_to1'.
-  eapply (Memory_le_Same _ mem mem') in MS_to1; auto.
+  subst to2 from.
+  replace (mem_map (SLL A) mem' NULLptr) with (@None (SLL A)) in *.
   congruence.
+  destruct MV2 as [EQnp [LTnp MV]]. auto.
+  
   subst to from.
   rename H into Sltc3.
   rename H0 into MS_to2.
   rename H1 into MS_to1'. 
-  eapply (Memory_le_Same _ mem mem') in MS_to1; auto.
+  replace (mem_map (SLL A) mem' NULLptr) with (@None (SLL A)) in *.
   congruence.
+  destruct MV2 as [EQnp [LTnp MV]]. auto.
 
   rename to into to1.
   rename from into from1.
@@ -213,15 +211,15 @@ Proof.
   rename H0 into MS_from1.
   eapply Acc_intro.
   intros [mem2 to2] Slt2.
-  destruct Slt2 as [MLE2 Sltc2].
+  destruct Slt2 as [MV2 [MLE2 Sltc2]].
   inversion Sltc2; clear Sltc2.
-  subst to from.
-  rename H into MS_to2.
-  rename H0 into MS_to1'.
+
+  subst to2 from.
+  rename H into MS_to1'.
   eapply (Memory_le_Same _ mem mem') in MS_to1; auto.
   replace v0 with v' in *; try congruence; clear v0.
-  replace to2 with next in *; try congruence; clear to2.
-  eapply IHSltc1. eauto.
+  replace NULLptr with next in *; try congruence.
+  eapply IHSltc1. auto. eauto.
 
   subst to from.
   rename H into Sltc3.
@@ -231,32 +229,43 @@ Proof.
   replace v0 with v' in *; try congruence; clear v0.
   replace to2 with next in *; try congruence; clear to2.
   clear MS_to1'.
-  eapply IHSltc1. eauto.
+  eapply IHSltc1. auto. eauto.
 Qed.  
 
 Lemma SLL_is_List_impl_SLL_lt:
   forall (A:Set) mem mem' a_after v_after a'_after,
+    Memory_Valid (SLL A) mem ->
     Memory_le (SLL A) mem mem' ->
     (exists l_after : list A, SLL_is_List A mem a_after l_after) ->
     mem_map (SLL A) mem a_after = Some (NODE A v_after a'_after) ->
     SLL_lt A (mem',a'_after) (mem,a_after).
 Proof.
-  intros A mem mem' a_after v_after a'_after MLE [l_after SiL] MS.
-  generalize mem' v_after a'_after MLE MS.
-  clear mem' v_after a'_after MLE MS.
-  induction SiL; intros mem' v_after a'_after MLE MS.
+  intros A mem mem' a_after v_after a'_after MV MLE [l_after SiL] MS.
+  generalize mem' v_after a'_after MV MLE MS.
+  clear mem' v_after a'_after MV MLE MS.
+  induction SiL; intros mem' v_after a'_after MV MLE MS.
+
+  destruct MV as [EQnp [LTnp MV]].
   congruence.
+  
   rename H into MS'.
   replace v with v_after in *; try congruence; clear v.
   replace a' with a'_after in *; try congruence; clear a'.
   clear MS'.
   unfold SLL_lt.
   inversion SiL; eauto.
+  subst mem0 a'_after l'.
+  split; auto.
+  split; auto.
+  eapply Sltc_NULL.
+  apply MS.
+
   subst mem0 a0 l'.
   rename H0 into MS'.
-  split; auto.
+  split. auto. split. auto.
   eapply Sltc_NODE.
   eapply IHSiL.
+  auto.
   apply MLE.
   apply MS'.
   apply MS'.
